examples-c/linked-lists/list.h
@@ -4,10 +4,9 @@ typedef struct struct_list {
   struct struct_list * tl;
 } *list;
 
-#define nil ((void*)0)
+#define NULL ((void*)0)
 
 /*@ predicate is_list(list l) reads l->tl */
-/*@ predicate llist(list l, plist pl) reads l->tl */
 /*@ predicate cyclic(list l) reads l->tl */
 
 /*@ logic plist rev(plist pl) */
@@ -17,22 +16,46 @@ typedef struct struct_list {
 /*@ logic StorePointerPair store_pointer_pair(list l) reads l->tl */
 
 
-
-/* @ inutile : predicate eq_list(plist l1, plist l2) */
-
-#if 0
 /* axioms for Simplify */
 
 /* axiom ll_order_wf : well_founded(ll_order) */
+
+/*@ logic plist nil() */ 
+/*@ logic plist cons(list p, plist l) */
+
+/*@ predicate lpath(list p1, plist l, list p2) reads p1->tl */
+
+/*@ axiom app_nil_end_ax :
+  @ \forall plist l; l == app(l,nil()) 
+  @*/
+
+/*@ axiom Path_null_ax : 
+  @ \forall list p; lpath(p,nil(),p)
+  @*/
+
+/*@ axiom Path_cons :
+  @ \forall list p1; \forall list p2;
+      \valid(p1) =>
+        \forall plist l;
+          lpath(p1->tl,l,p2) => lpath(p1,cons(p1,l),p2)
+*/
+
+/** [(llist t p l)]: there is a (finite) linked list starting from pointer [p]
+    using links in store [t], and this list of pointers is [l] */
+/*@ predicate llist(list p, plist l) { lpath(p,l,\null) } */ 
 
 /*@ axiom is_list_llist_ax :
     \forall list p;
      is_list(p) => \exists plist l; llist(p,l) */
 
-/*@ axiom llist_function_ax :
+/* axiom llist_function_ax :
     \forall plist l1; \forall plist l2; \forall list p;
     llist(p,l1) => llist(p,l2) => eq_list(l1,l2) */
 
-/*@ axiom eq_list_def : \forall plist x; \forall plist y;
-    x==y => eq_list(x,y) */
-#endif
+/*@ axiom disjoint_nil1 :
+  \forall plist l; disjoint(l,nil()) */
+
+/*@ axiom disjoint_nil2 :
+  \forall plist l; disjoint(nil(),l) */
+   
+
